Also construct relatedness proofs in reified

src/Specific/GF25519Reflective/Reified/rebuild-reified.py
@@ -1,0 +1,15 @@
+#!/usr/bin/env python2.7
+from __future__ import with_statement
+
+for name, opkind in ([(name, 'binop') for name in ('Add', 'Carry_Add', 'Sub', 'Carry_Sub', 'Mul')]
+                     + [('Opp', 'unop'), ('Carry_Opp', 'unop'), ('Freeze', 'unop'),
+                        ('Ge_Modulus', 'unop_FEToZ'), ('Pack', 'unop_FEToWire'), ('Unpack', 'unop_WireToFE')]):
+    lname = name.lower()
+    with open(name.replace('_', '') + '.v', 'w') as f:
+        f.write(r"""Require Import Crypto.Specific.GF25519Reflective.Common.
+
+Definition r%(lname)sZ_sig : rexpr_%(opkind)s_sig %(lname)s. Proof. reify_sig. Defined.
+Definition r%(lname)sW := Eval vm_compute in rword_of_Z r%(lname)sZ_sig.
+Lemma r%(lname)sW_correct_and_bounded_gen : correct_and_bounded_genT r%(lname)sW r%(lname)sZ_sig.
+Proof. rexpr_correct. Qed.
+""" % locals())
