src/Specific/GF25519Reflective/Reified/Freeze.v
@@ -1,3 +1,6 @@
 Require Import Crypto.Specific.GF25519Reflective.Common.
 
 Definition rfreezeZ_sig : rexpr_unop_sig freeze. Proof. reify_sig. Defined.
+Definition rfreezeW := Eval vm_compute in rword_of_Z rfreezeZ_sig.
+Lemma rfreezeW_correct_and_bounded_gen : correct_and_bounded_genT rfreezeW rfreezeZ_sig.
+Proof. rexpr_correct. Qed.
