src/Specific/GF25519Reflective/Reified/GeModulus.v
@@ -1,3 +1,6 @@
 Require Import Crypto.Specific.GF25519Reflective.Common.
 
 Definition rge_modulusZ_sig : rexpr_unop_FEToZ_sig ge_modulus. Proof. reify_sig. Defined.
+Definition rge_modulusW := Eval vm_compute in rword_of_Z rge_modulusZ_sig.
+Lemma rge_modulusW_correct_and_bounded_gen : correct_and_bounded_genT rge_modulusW rge_modulusZ_sig.
+Proof. rexpr_correct. Qed.
