src/Specific/GF25519Reflective/Reified/Opp.v
@@ -1,3 +1,6 @@
 Require Import Crypto.Specific.GF25519Reflective.Common.
 
 Definition roppZ_sig : rexpr_unop_sig opp. Proof. reify_sig. Defined.
+Definition roppW := Eval vm_compute in rword_of_Z roppZ_sig.
+Lemma roppW_correct_and_bounded_gen : correct_and_bounded_genT roppW roppZ_sig.
+Proof. rexpr_correct. Qed.
