src/Specific/GF25519Reflective/Reified/Pack.v
@@ -1,3 +1,6 @@
 Require Import Crypto.Specific.GF25519Reflective.Common.
 
 Definition rpackZ_sig : rexpr_unop_FEToWire_sig pack. Proof. reify_sig. Defined.
+Definition rpackW := Eval vm_compute in rword_of_Z rpackZ_sig.
+Lemma rpackW_correct_and_bounded_gen : correct_and_bounded_genT rpackW rpackZ_sig.
+Proof. rexpr_correct. Qed.
