src/Specific/GF25519Reflective/Reified/Sub.v
@@ -1,3 +1,6 @@
 Require Import Crypto.Specific.GF25519Reflective.Common.
 
 Definition rsubZ_sig : rexpr_binop_sig sub. Proof. reify_sig. Defined.
+Definition rsubW := Eval vm_compute in rword_of_Z rsubZ_sig.
+Lemma rsubW_correct_and_bounded_gen : correct_and_bounded_genT rsubW rsubZ_sig.
+Proof. rexpr_correct. Qed.
