src/Specific/GF25519Reflective/Reified/Unpack.v
@@ -1,3 +1,6 @@
 Require Import Crypto.Specific.GF25519Reflective.Common.
 
 Definition runpackZ_sig : rexpr_unop_WireToFE_sig unpack. Proof. reify_sig. Defined.
+Definition runpackW := Eval vm_compute in rword_of_Z runpackZ_sig.
+Lemma runpackW_correct_and_bounded_gen : correct_and_bounded_genT runpackW runpackZ_sig.
+Proof. rexpr_correct. Qed.
